\section{Squeezed states}
Lets define the squeeze operator 
\begin{align*}
    \text{Squeezing state}\qquad\ket{\xi,0}=\hS(\xi)\ket{0},\quad\text{with}\quad\hS(\xi)=e^{\frac{1}{2}(\xi^*\ha^2-\xi\ha^{\dagger2})},\quad\xi\in\mathbb{C}.
\end{align*}
Lets use it to compute the expectation value for the quadrature operators.
\begin{align*}
    \braket{\xi,0|\hX_1|\xi,0}&=\braket{0|\hS^\dagger(\xi)\left(\frac{\ha+\ha^\dagger}{2}\right)\hS(\xi)|0}=\frac{1}{2}\braket{0|(\hS^\dagger\ha\hS+\hS^\dagger\ha^\dagger\hS)|0}.
\end{align*}
We define displaced ladder operators as
\begin{align*}
    \tilde{a}=\hS^\dagger(\xi)\ha\hS(\xi),\quad\xi=re^{i\phi}.
\end{align*}
Using the BCH formula 
\begin{align*}
    e^LAe^{-L}=A+[L,A]+\frac{1}{2!}[L,[L,A]]+\cdots
\end{align*}
and $A=\ha$ with $L=-\frac{1}{2}(\xi^*\ha^2-\xi\ha^{\dagger2})$ allow us to express the squeezing ladder operator 
\begin{align}
    \text{Squeezing ladder operators}\qquad
    \highlight{
    \begin{array}{l}
        \tilde{a}=\hS^\dagger(\xi)\ha\hS(\xi)=\ha\cosh(r)-\ha^\dagger e^{i\phi}\sinh(r)\\
        \tilde{a}^\dagger=S(\xi)^\dagger\ha^\dagger\hS(\xi)=\ha^\dagger\cosh(r)-\ha e^{i\phi}\sinh(r).
    \end{array}}
\end{align}
We have used several orders. Its derivative wrt $r$ is:
\begin{align*}
    \frac{d\ha}{dr}=\ha\sinh(r)-\ha^\dagger e^{i\phi}\cosh(r)=-e^{i\phi}\tilde{a}^\dagger,\quad\frac{d\tilde{a}^\dagger}{dr}=-e^{-i\phi}\tilde{a}.
\end{align*} 
Taking another derivative yields:
\begin{align*}
    \frac{d^2\tilde{a}}{dr^2}=\tilde{a}.
\end{align*}
Now we can continue the expectation of the quadrature:
\begin{align*}
    \braket{\hX_1}&=\frac{1}{2}\braket{0|(\hS^\dagger\ha\hS+\hS^\dagger\ha^\dagger\hS)|0}=\frac{1}{2}\braket{0|\left[\tilde{a}+\tilde{a}^\dagger\right]|0}\\
    &=\frac{1}{2}\braket{0|[\ha\cosh(r)-e^{i\phi}\ha^\dagger\sinh(r)+\ha^\dagger\cosh(r)-e^{-i\phi}\sinh(r)]|0}=0.\\
    \braket{\hX_2}&=\text{similarly}=0.
\end{align*}
We can do the same for the operator square:
\begin{align*}
    \braket{\hX_1^2}&=\frac{1}{4}\braket{0|\hS^\dagger(\xi)[(\ha+\ha^\dagger)(\ha+\ha^\dagger)]\hS(\xi)|0}=\frac{1}{4}\braket{0|\hS^\dagger(\ha+\ha^\dagger)\hS\hS^\dagger(\ha+\ha^\dagger)\hS|0}\\
    &=\frac{1}{4}\braket{0|(\tilde{a}+\tilde{a}^\dagger)(\tilde{a}+\tilde{a}^\dagger)|0}=\frac{1}{4}\braket{0|e^{-2r}(\ha+\ha^\dagger)^2|0}=\frac{e^{-2r}}{4}.
\end{align*}
Similarly we can obtain the respective quantities for $\hX_2$ and the uncertainties are:
\begin{align*}
    \braket{\hX_1}=\braket{\hX_2}=0 \Longrightarrow
    \Delta\hX_1=\frac{e^{-r}}{2},\quad\Delta\hX_2=\frac{e^r}{2}.
\end{align*}
%%
\subsection{Displaced squeezing state}
Now,
\begin{align*}
    \shortstack{Displaced squeezing state}\qquad\ket{\xi,\alpha}=\hD(\alpha)\hS(\xi)\ket{0}.
\end{align*}
Now, the operators are:
\begin{align}
    \shortstack{Displaced squeezing\\operator}\qquad\highlight{
    \begin{array}{l}
        \tilde{a}=\hS^\dagger(\xi)\hD^\dagger(\alpha)\ha\hD(\alpha)\hS(\xi)=\cosh(r)\ha-e^{i\phi}\sinh(r)\ha^\dagger+\alpha,\\
        \tilde{a}^\dagger=\hS^\dagger(\xi)\hD^\dagger(\alpha)\ha^\dagger\hD(\alpha)\hS(\xi)=\cosh(r)\ha^\dagger-e^{-i\phi}\sinh(r)\ha+\alpha^*.
    \end{array}}
\end{align}
The expected number of photons in a displaced squeezed state is:
\begin{align*}
    \braket{0|\tilde{a}^\dagger\tilde{a}|0}=\braket{0|[\cosh(r)\ha^\dagger-e^{-i\phi}\sinh(r)\ha+\alpha^*][\cosh(r)\ha-e^{i\phi}\sinh(r)\ha^\dagger+\alpha]|0}=\sinh^2|\xi|+|\alpha|^2.
\end{align*}
The expected value in the quadrature value is:
\begin{align*}
    \braket{\xi,\alpha|\hX_1|\xi,\alpha}&=\braket{0|\hS^\dagger\hD^\dagger\hX_1\hD\hS|0}=\braket{0|\hS^\dagger\hD^\dagger(\frac{\ha+\ha^\dagger}{2})\hD\hS|0}=
    \frac{1}{2}\braket{0|(\tilde{a}+\tilde{a}^\dagger)|0}\\
    &=\frac{1}{2}\braket{0|[\cosh(r)\ha-e^{i\phi}\sinh(r)\ha^\dagger+\alpha+\cosh(r)\ha^\dagger-e^{-i\phi}\sinh(r)\ha+\alpha^*]|0}=\re{\alpha}.\\
    \braket{\xi,\alpha|\hX_2|\xi,\alpha}&=\im{\alpha}.
\end{align*}

On the other hand, the quadrature uncertainties are:
\begin{align*}
    \Delta\hX_1^2&=\braket{\xi,\alpha|\hX_1^2|\xi,\alpha}-\braket{\xi,\alpha|\hX_1|\xi,\alpha}^2=\braket{0|\hS^\dagger\hD^\dagger\hX_1\hD\hS\hS^\dagger\hD^\dagger\hX_1\hD\hS|0}-\re{\alpha}^2\\
    &=\braket{0|\left(\frac{\tilde{a}+\tilde{a}^\dagger}{2}\right)\left(\frac{\tilde{a}+\tilde{a}^\dagger}{2}\right)|0}-\re{\alpha}^2\\
    &=\frac{1}{4}\braket{0|[\cosh(r)\ha-e^{i\phi}\sinh(r)\ha^\dagger+\alpha+\cosh(r)\ha^\dagger-e^{-i\phi}\sinh(r)\ha+\alpha^*]^2|0}-\re{\alpha}^2\\
    &=\frac{1}{4}(\cosh^2(r)+\sinh^2(r)-2\cosh(r)\sinh(r)\cos\phi)+\re(\alpha)^2-\re(\alpha)^2\\
    \Delta\hX_1^2&=\frac{1}{4}[\cosh^2(r)+\sinh^2(r)-2\cosh(r)\sinh(r)\cos(\phi)].\\
    \Delta\hX_2^2&=\frac{1}{4}[\cosh^2(r)+\sinh^2(r)+2\cosh(r)\sinh(r)\cos(\phi)].
\end{align*}

\begin{figure}[htbp]
    \centering
    \begin{subfigure}{.45\columnwidth}
        \centering
        \includegraphics[width=\columnwidth]{PartOne/ChapterOne/figures/displacedsqueezedstate.png}
        \caption{}
    \end{subfigure}
    \hfill
    \begin{subfigure}{.45\columnwidth}
        \centering
        \includegraphics[width=\columnwidth]{PartOne/ChapterOne/figures/displacedsqueezedstate_b.png}
        \caption{}
    \end{subfigure}
    \caption{}
\end{figure}